%#BIBTEX semiautotex.sh -b note_LF_DEM
\documentclass[12pt]{article}
\usepackage{amsmath,amssymb}
\usepackage{bm}
%\usepackage{hyperref}
\usepackage[pdftex]{graphicx}	% required for `\includegraphics' (yatex added)
\usepackage{datetime}
\usepackage{natbib}

\oddsidemargin -1.2cm
\evensidemargin -1.2cm
\textwidth 18cm
\headheight 1.0in
\topmargin -3.5cm
\textheight 22cm
\bibliographystyle{unsrtnat}
\newcommand{\figref}[1]{\figurename ~\ref{#1}}
\newcommand{\tens}[1]{\bm{\mathsf{#1}}}
\title{Title}
\date{\shortdate\today \, \ampmtime }
\author{R. Seto, R. Mari}
\begin{document}
\maketitle


\subsection*{The leading lubrication forces}

\begin{equation}
 \begin{pmatrix}
  \bm{F} \\ \bm{T} \\ \bm{S}
 \end{pmatrix}
 =
- \mu
\begin{pmatrix}
 \tens{A} &  \tilde{\tens{B}} &  \tilde{\tens{G}} \\
 \tens{B} &  \tens{C} &  \tilde{\tens{H}} \\
 \tens{G} &  \tens{H} &  \tens{M} \\
\end{pmatrix}
 \begin{pmatrix}
  \bm{U}-\bm{U}_{\infty} \\ \bm{\Omega} - \bm{\Omega}_{\infty}
 \\ -\bm{E}_{\infty}
 \end{pmatrix}
\end{equation}
\begin{equation}
 \bm{F}
= 
\begin{pmatrix}
 \bm{F}_\alpha \\  \bm{F}_\beta
\end{pmatrix}
,\quad
 \bm{T}
= 
\begin{pmatrix}
 \bm{T}_\alpha \\  \bm{T}_\beta
\end{pmatrix}
,\quad
 \bm{S}
= 
\begin{pmatrix}
 \bm{S}_\alpha \\  \bm{S}_\beta
\end{pmatrix}
,\quad
 \bm{U}
= 
\begin{pmatrix}
 \bm{U}_\alpha \\  \bm{U}_\beta
\end{pmatrix}
,\quad
 \bm{\Omega}
= 
\begin{pmatrix}
 \bm{\Omega}_\alpha \\  \bm{\Omega}_\beta
\end{pmatrix}
\end{equation}
\begin{equation}
 \tens{A}
 =
\begin{pmatrix}
  \tens{A}_{\alpha\alpha} & \tens{A}_{\alpha\beta} \\
  \tens{A}_{\beta\alpha} & \tens{A}_{\beta\beta} 
\end{pmatrix}
\end{equation}
Similarly for 
$\tens{B}$, $\tens{C}$, $\tens{G}$,
$\tens{H}$, $\tens{M}$, 
$\tilde{\tens{B}}$, $\tilde{\tens{C}}$, $\tilde{\tens{H}}$.
%

\paragraph{Symmetries:}
2-indeces:
\begin{equation}
 A_{ij}^{\alpha\beta} =  A_{ji}^{\beta\alpha}
\end{equation}
3-indeces:
\begin{equation}
 G_{ijk}^{\alpha\beta} =   G_{jik}^{\alpha\beta} , \quad 
 G_{iik}^{\alpha\beta} =   H_{iik}^{\alpha\beta}  = 0, \quad 
 \tilde{G}_{ijk}^{\alpha\beta}  =  G_{jki}^{\beta\alpha} 
\end{equation}
4-indeces:
\begin{equation}
 M_{iikl}^{\alpha\beta} = 0,
\quad 
 M_{iikl}^{\alpha\beta} =  M_{lkij}^{\beta\alpha} 
\end{equation}

\paragraph{Adimensional tensors:}
\begin{equation}
 \hat{\tens{A}}_{\alpha\beta}
= \frac{\tens{A}_{\alpha\beta}}{3\pi(a_{\alpha} + a_{\beta})},
\quad
 \hat{\tens{B}}_{\alpha\beta}
= \frac{\tens{B}_{\alpha\beta}}{\pi(a_{\alpha}+ a_{\beta})^2},
\quad
 \hat{\tens{C}}_{\alpha\beta}
= \frac{\tens{C}_{\alpha\beta}}{\pi(a_{\alpha}+ a_{\beta})^3}
\end{equation}

\begin{equation}
 \hat{\tens{G}}_{\alpha\beta}
= \frac{\tens{G}_{\alpha\beta}}{3\pi(a_{\alpha} + a_{\beta})},
\quad
 \hat{\tens{H}}_{\alpha\beta}
= \frac{\tens{H}_{\alpha\beta}}{\pi(a_{\alpha}+ a_{\beta})^3},
\quad
 \hat{\tens{M}}_{\alpha\beta}
= \frac{\tens{M}_{\alpha\beta}}{(5/6)\pi(a_{\alpha}+ a_{\beta})^3}
\end{equation}

\paragraph{Variables:}
\begin{equation}
 \bm{r} = \bm{r}_\alpha - \bm{r}_\beta, \quad
 \bm{e} = \frac{\bm{r}}{r}
\end{equation}
\begin{equation}
  s = \frac{2r}{a_{\alpha}+ a_{\beta}}, \quad
 \lambda = \frac{a_\beta}{a_\alpha}, \quad
\xi \equiv \frac{r -  (a_\alpha + a_\beta)}{(a_{\alpha}+ a_{\beta})/2} 
\end{equation}


\paragraph{Scalar functions}

\begin{equation}
  \hat{A}_{ij}^{\alpha \beta}
  = 
  X_{\alpha \beta}^{A} \bm{e}_i \bm{e}_j
  +
  Y_{\alpha \beta}^{A} (\delta_{ij} - e_i e_j)
\end{equation}

\begin{equation}
  \hat{B}_{ij}^{\alpha \beta}
  = 
  Y_{\alpha \beta}^{B}   \varepsilon_{ijk} e_k
\end{equation}

\begin{equation}
  \hat{C}_{ij}^{\alpha \beta}
  = 
  X_{\alpha \beta}^{C} \bm{e}_i \bm{e}_j
  +
  Y_{\alpha \beta}^{C} (\delta_{ij} - e_i e_j)
\end{equation}

\begin{equation}
 \hat{G}_{ijk}^{\alpha \beta}
 = 
X_{\alpha\beta}^{G} 
\left(e_ie_j - \frac{1}{3}\delta_{ij}\right)
+
Y_{\alpha\beta}^{G}
\left(
e_i \delta_{jk} + e_j \delta_{ik} - 2 e_i e_j e_k
\right)
\end{equation}
\begin{equation}
 \hat{H}_{ij}^{\alpha\beta}
 = Y_{\alpha\beta}^{H}
(e_i \varepsilon_{jkm} e_m 
+ e_j \varepsilon_{ikm} e_m )
\end{equation}
\begin{align}
 \hat{M}_{ijkl}^{\alpha\beta}
& = X_{\alpha\beta}^{M}
\frac{3}{2}
 \left(e_i e_j
 - \frac{1}{3} \delta_{ij}
\right)
 \left(e_k e_l
 - \frac{1}{3} \delta_{kl}
\right) \\
& \quad
+ 
Y_{\alpha\beta}^{M}
\frac{1}{2}
\left(
e_i \delta_{jl} e_k
+
e_j \delta_{il} e_k
+
e_i \delta_{jk} e_l
+
e_j \delta_{ik} e_l
-
4 e_i e_j e_k e_l
\right) \\
&\quad
+ Z_{\alpha\beta}^{M}
\frac{1}{2}
\left(
\delta_{ik}\delta_{jl}
+
\delta_{jk}\delta_{il}
-
\delta_{ij}\delta_{kl}
+
e_i e_j \delta_{kl} 
+
\delta_{ij} e_k e_l
+
e_i e_j e_k e_l \right.\\
&\qquad \qquad \quad
\left.
- 
e_i \delta_{jl} e_k
-
e_j \delta_{il} e_k
-
e_i \delta_{jk} e_l
-
e_j \delta_{ik} e_l
\right)
\end{align}

\paragraph{Leading terms}

The leading terms are $\xi^{-1}$ with 




These are only $X$ functions.

$Y$ functions scale as $\ln \xi^{-1}$.


\begin{equation}
 g_1 (\lambda)
= \frac{2\lambda^2}{(1+\lambda)^3}
\end{equation}

\begin{equation}
 X_{\alpha\alpha}^{A}
= 
g_1(\lambda) \xi^{-1}, \quad
 X_{\alpha\beta}^{A}
= 
-\frac{2}{1+\lambda}g_1(\lambda) \xi^{-1}
\end{equation}

\begin{equation}
 X_{\alpha\alpha}^{C} 
\sim
 X_{\alpha\beta}^{C}
\sim
\mathcal{O}(1) + \mathcal{O}(\xi \ln \xi^{-1}).
\end{equation}

\begin{equation}
 X_{\alpha\alpha}^{G}
= \frac{3}{2}g_1(\lambda) \xi^{-1}
\quad 
 X_{\alpha \beta}^{G}
= \frac{-6}{(1+\lambda)^2}
g_1 (\lambda) \xi^{-1}
\end{equation}

\begin{equation}
 X_{\alpha \alpha}^{M}
=
\frac{3}{5} g_1(\lambda) \xi^{-1},
\quad
 X_{\alpha \beta}^{M}
=
\frac{8\lambda}{(1+\lambda)^3} g_1(\lambda) \xi^{-1}.
\end{equation}



\newpage

\subsection*{Hydrodynamic force}

One-body limit:
\begin{align}
 \bm{F}_i^{\mathrm{self}} &= 
-6 \pi \mu a ( \bm{v}_i - \bm{U}^{\infty} (\bm{r}_i) ) \\
 \bm{T}_i^{\mathrm{self}} &= 
-8 \pi \mu a^3 ( \bm{\omega}_i - \bm{\Omega}^{\infty})
\end{align}

\citet{Melrose_2004a} uses 
the leading squeeze mode of lubrication force:
\begin{align}
 \bm{F}_{ij}^{\mathrm{pair}}
&=
- \alpha_{\mathrm{n}}(h_{ij})
\bigl\{
(\bm{v}_i - \bm{v}_j)
\cdot \bm{n}_{ij}
\bigr\}
\bm{n}_{ij} \\
 \bm{T}_{ij}^{\mathrm{pair}}
&=
\bm{0},
\end{align}
where
\begin{equation}
 \alpha_{\mathrm{n}}(h_{ij}) = 
\frac{3 \pi \mu a^2}{2 h_{\ij}}.
\end{equation}
Note: We should check the model of \citet{Ball_1997,Melrose_2004a}.
%
We need to understand the difference from FTS version~\citet{Jeffrey_1992}.


Hydrodynamic interaction acting on particle $i$
is given by
\begin{align}
\bm{F}_i^{\mathrm{H}}
&=
\bm{F}_i^{\mathrm{self}}
+
\sum_j
\bm{F}_{ij}^{\mathrm{pair}} \\
\bm{T}_i^{\mathrm{H}}
&=
\bm{T}_i^{\mathrm{self}}
\end{align}




\newpage
\subsection*{Dimensionless equations}

The unit of length, velocity and force 
are given:
$L_0 = a$,  $v_0 = a \dot{\gamma}$, and $F_0 \equiv 6 \pi \mu a v_0$.

The dimensionless variables are introduced:
$\tilde{h}_{ij} = h_{ij} / L_0$,
$\tilde{\bm{v}}_i = \bm{v}_i / U_0$,
and $\tilde{\bm{F}}_{ij}^{\mathrm{pair}} = \bm{F}_{ij}^{\mathrm{pair}} / F_0$.

The relations are written as follows:
\begin{equation}
 \tilde{\bm{F}}_i^{\mathrm{self}} = 
-( \tilde{\bm{v}}_i - 
\tilde{\bm{U}}^{\infty} 
(\tilde{\bm{r}}_i) )
\end{equation}
\begin{equation}
 \tilde{\bm{F}}_{ij}^{\mathrm{pair}}
= 
- \frac{1}{4 \tilde{h}_{ij}}
\bigl\{
(\tilde{\bm{v}}_i-
\tilde{\bm{v}}_i)\cdot
\bm{n}_{ij}
\bigr\}\bm{n}_{ij}
\end{equation}

\begin{equation}
 \bm{U}^{\infty}(\bm{r})
 = 
 \dot{\gamma} z \bm{e}_{x}
\end{equation}
\begin{equation}
\Longrightarrow
  \tilde{\bm{U}}^{\infty}(\tilde{\bm{r}})
 = 
 \dot{\gamma} z \bm{e}_{x} / U_0
=  \dot{\gamma} z \bm{e}_{x} / (\dot{\gamma} a)
= \tilde{z} \bm{e}_{x} 
\end{equation}


\newpage
\subsection*{Matrix form}
\begin{align}
 \bm{F}_{ij}^{\mathrm{pair}}
&= 
- \frac{1}{4 h_{ij}}
\bigl\{
(\bm{v}_i-
\bm{v}_j)\cdot
\bm{n}_{ij}
\bigr\}\bm{n}_{ij} \\
&=
- \frac{1}{4 h_{ij}}
\Bigl[
\bigl\{
(\bm{v}_i- \bm{U}^{\infty}_i)-
(\bm{v}_j- \bm{U}^{\infty}_j)
+ \bm{U}^{\infty}_i 
- \bm{U}^{\infty}_j
\bigr\}\cdot
\bm{n}_{ij}
\Bigr]
\bm{n}_{ij}
\end{align}

$\Delta \bm{v} \equiv (\bm{v}- \bm{U}^{\infty})$
\begin{align}
\Delta \bm{v} \cdot
\bm{n} \bm{n}
= &
(\Delta v_x n_x 
+\Delta v_y n_y
+\Delta v_z n_z) n_x \bm{i}\\
& 
+ (\Delta v_x n_x 
+\Delta v_y n_y
+\Delta v_z n_z) n_y \bm{j}\\
&
+ (\Delta v_x n_x 
+\Delta v_y n_y
+\Delta v_z n_z) n_z \bm{k} \\
=&
\begin{pmatrix}
 n_x n_x &   n_y n_x &   n_z n_x \\
 n_x n_y &   n_y n_y &   n_z n_y \\
 n_x n_z &   n_y n_z &   n_z n_z 
\end{pmatrix}
\begin{pmatrix}
 \Delta v_x \\
 \Delta v_y \\
 \Delta v_z 
\end{pmatrix} 
\\
=&\bm{n} \otimes \bm{n} \Delta \bm{v}
\end{align}

\begin{align}
  \bm{F}_i  &= 
  -  \Delta \bm{v}_i 
  - \sum_j
  \left(
    \frac{1}{4h_{ij}} \bm{n}_{ij} \otimes \bm{n}_{ij} \Delta \bm{v}_i
    - \frac{1}{4h_{ij}} \bm{n}_{ij} \otimes \bm{n}_{ij} \Delta \bm{v}_j 
    + \frac{1}{4h_{ij}}  
 \bm{n}_{ij} \otimes \bm{n}_{ij} (\bm{U}_i^{\infty}-\bm{U}_j^{\infty})
  \right) \\
  &=
 -  \Delta \bm{v}_i 
  - \sum_j
  \left(
    \frac{1}{4h_{ij}} \bm{n}_{ij} \otimes \bm{n}_{ij} \Delta \bm{v}_i
    - \frac{1}{4h_{ij}} \bm{n}_{ij} \otimes \bm{n}_{ij} \Delta \bm{v}_j
    + \frac{1}{4h_{ij}}  
 \bm{n}_{ij} \otimes \bm{n}_{ij} (\bm{U}_i^{\infty}-\bm{U}_j^{\infty})
\right)
  \end{align}


\begin{align}
\begin{pmatrix}
\vdots \\ \bm{F}_i \\ \vdots \\ \bm{F}_j \\  \vdots  
\end{pmatrix}
& =
\begin{pmatrix}
\vdots \\
\bm{F}_{i}^{\mathrm{self}} +  \bm{F}_{ij}^{\mathrm{pair}}  
\\ \vdots \\ 
\bm{F}_{j}^{\mathrm{self}} +  \bm{F}_{ji}^{\mathrm{pair}}  
\\  \vdots  
\end{pmatrix} \\
&=
-
\begin{pmatrix}
\cdots & \cdots & \cdots & \cdots & \cdots\\
\cdots & 1 + \frac{1}{4h_{ij}}\bm{n}_{ij} \otimes \bm{n}_{ij}  
& \cdots & -\frac{1}{4h_{ij}}\bm{n}_{ij} \otimes \bm{n}_{ij}   & \cdots\\
\cdots & \cdots & \cdots & \cdots & \cdots\\
\cdots & -\frac{1}{4h_{ji}}\bm{n}_{ji} \otimes \bm{n}_{ji} & \cdots 
& 1 + \frac{1}{4h_{ji}}\bm{n}_{ji} \otimes \bm{n}_{ji} 
 & \cdots \\
\cdots & \cdots & \cdots & \cdots & \cdots 
\end{pmatrix}
\begin{pmatrix}
\vdots \\
\Delta \bm{v}_i \\ 
\vdots \\
\Delta \bm{v}_j \\
\vdots 
\end{pmatrix} \\
& \quad 
+ 
\begin{pmatrix}
\vdots \\
-\frac{1}{4h_{ij}}
 \frac{(z_i - z_j )(x_i-x_j)}{r_{ij}} 
 \bm{n}_{ij} \\
\vdots \\
-\frac{1}{4h_{ji}} 
 \frac{(z_j - z_i )(x_j - x_i)}{r_{ji}} 
\bm{n}_{ji} \\
\vdots 
\end{pmatrix} 
\end{align}

\newpage
\subsection*{Force balance equation}





\newpage
\bibliography{/Users/seto/Dropbox/Papers/rse}
\end{document}